dist/gcc-compatible/lib/Hacl_HPKE_Curve64_CP256_SHA256_bindings.ml
@@ -10,7 +10,6 @@ module Bindings(F:Cstubs.FOREIGN) =
                  (ocaml_bytes @->
                     (ocaml_bytes @->
                        (uint32_t @-> (ocaml_bytes @-> (returning uint32_t))))))))
-      
     let hacl_HPKE_Curve64_CP256_SHA256_setupBaseR =
       foreign "Hacl_HPKE_Curve64_CP256_SHA256_setupBaseR"
         (ocaml_bytes @->
@@ -18,7 +17,6 @@ module Bindings(F:Cstubs.FOREIGN) =
               (ocaml_bytes @->
                  (ocaml_bytes @->
                     (uint32_t @-> (ocaml_bytes @-> (returning uint32_t)))))))
-      
     let hacl_HPKE_Curve64_CP256_SHA256_sealBase =
       foreign "Hacl_HPKE_Curve64_CP256_SHA256_sealBase"
         (ocaml_bytes @->
@@ -28,7 +26,6 @@ module Bindings(F:Cstubs.FOREIGN) =
                     (uint32_t @->
                        (ocaml_bytes @->
                           (ocaml_bytes @-> (returning uint32_t))))))))
-      
     let hacl_HPKE_Curve64_CP256_SHA256_openBase =
       foreign "Hacl_HPKE_Curve64_CP256_SHA256_openBase"
         (ocaml_bytes @->
@@ -38,5 +35,4 @@ module Bindings(F:Cstubs.FOREIGN) =
                     (uint32_t @->
                        (ocaml_bytes @->
                           (ocaml_bytes @-> (returning uint32_t))))))))
-      
   end
