code/streaming/Hacl.Streaming.Functor.fsti
@@ -31,18 +31,23 @@ let uint32 = Lib.IntTypes.uint32
 /// ===============
 
 [@CAbstractStruct]
-val state_s (#index: Type0) (c: block index) (i: index): Type0
+val state_s (#index: Type0) (c: block index) (i: index) (t: Type0 { t == c.state i }): Type0
 
-let state #index (c: block index) (i: index) = B.pointer (state_s c i)
+/// State is equipped with a superfluous type-level parameter to ensure ML-like
+/// prenex polymorphism and hence low-level monomorphization via KreMLin.
+///
+/// Run-time functions MUST take t as a parameter. Proof-level functions are
+/// welcome to instantiate it directly with ``c.state i``.
+let state #index (c: block index) (i: index) (t: Type0 { t == c.state i }) = B.pointer (state_s c i t)
 
-val freeable (#index: Type0) (c: block index) (i: index) (h: HS.mem) (p: state c i): Type0
+val freeable (#index: Type0) (c: block index) (i: index) (h: HS.mem) (p: state c i (c.state i)): Type0
 
-let preserves_freeable #index (c: block index) (i: index) (s: state c i) (h0 h1: HS.mem): Type0 =
+let preserves_freeable #index (c: block index) (i: index) (s: state c i (c.state i)) (h0 h1: HS.mem): Type0 =
   freeable c i h0 s ==> freeable c i h1 s
 
-val footprint_s (#index: Type0) (c: block index) (i: index) (h: HS.mem) (s: state_s c i): GTot B.loc
+val footprint_s (#index: Type0) (c: block index) (i: index) (h: HS.mem) (s: state_s c i (c.state i)): GTot B.loc
 
-let footprint (#index: Type0) (c: block index) (i: index) (m: HS.mem) (s: state c i) =
+let footprint (#index: Type0) (c: block index) (i: index) (m: HS.mem) (s: state c i (c.state i)) =
   B.(loc_union (loc_addr_of_buffer s) (footprint_s c i m (B.deref m s)))
 
 /// Invariants
@@ -56,7 +61,7 @@ let loc_includes_union_l_footprint_s
   (c: block index)
   (i: index)
   (m: HS.mem)
-  (l1 l2: B.loc) (s: state_s c i)
+  (l1 l2: B.loc) (s: state_s c i (c.state i))
 : Lemma
   (requires (
     B.loc_includes l1 (footprint_s c i m s) \/ B.loc_includes l2 (footprint_s c i m s)
@@ -65,9 +70,9 @@ let loc_includes_union_l_footprint_s
   [SMTPat (B.loc_includes (B.loc_union l1 l2) (footprint_s c i m s))]
 = B.loc_includes_union_l l1 l2 (footprint_s c i m s)
 
-val invariant_s (#index: Type0) (c: block index) (i: index) (h: HS.mem) (s: state_s c i): Type0
+val invariant_s (#index: Type0) (c: block index) (i: index) (h: HS.mem) (s: state_s c i (c.state i)): Type0
 
-let invariant #index (c: block index) (i: index) (m: HS.mem) (s: state c i) =
+let invariant #index (c: block index) (i: index) (m: HS.mem) (s: state c i (c.state i)) =
   B.live m s /\
   B.(loc_disjoint (loc_addr_of_buffer s) (footprint_s c i m (B.deref m s))) /\
   invariant_s c i m (B.get m s 0)
@@ -76,7 +81,7 @@ val invariant_loc_in_footprint
   (#index: Type0)
   (c: block index)
   (i: index)
-  (s: state c i)
+  (s: state c i (c.state i))
   (m: HS.mem)
 : Lemma
   (requires (invariant c i m s))
@@ -127,9 +132,9 @@ val invariant_loc_in_footprint
 ///
 ///                                            JP (20190607)
 
-val seen: #index:Type0 -> c:block index -> i:index -> h:HS.mem -> s:state c i -> GTot bytes
+val seen: #index:Type0 -> c:block index -> i:index -> h:HS.mem -> s:state c i (c.state i) -> GTot bytes
 
-val seen_bounded: #index:Type0 -> c:block index -> i:index -> h:HS.mem -> s:state c i -> Lemma
+val seen_bounded: #index:Type0 -> c:block index -> i:index -> h:HS.mem -> s:state c i (c.state i) -> Lemma
   (requires (
     invariant c i h s))
   (ensures (
@@ -148,7 +153,7 @@ val seen_bounded: #index:Type0 -> c:block index -> i:index -> h:HS.mem -> s:stat
 /// to always heap allocating, then we could conceivably have a single framing
 /// lemma.
 
-val frame_invariant: #index:Type0 -> c:block index -> i:index -> l:B.loc -> s:state c i -> h0:HS.mem -> h1:HS.mem -> Lemma
+val frame_invariant: #index:Type0 -> c:block index -> i:index -> l:B.loc -> s:state c i (c.state i) -> h0:HS.mem -> h1:HS.mem -> Lemma
   (requires (
     invariant c i h0 s /\
     B.loc_disjoint l (footprint c i h0 s) /\
@@ -158,7 +163,7 @@ val frame_invariant: #index:Type0 -> c:block index -> i:index -> l:B.loc -> s:st
     footprint c i h0 s == footprint c i h1 s))
   [ SMTPat (invariant c i h1 s); SMTPat (B.modifies l h0 h1) ]
 
-val frame_seen: #index:Type0 -> c:block index -> i:index -> l:B.loc -> s:state c i -> h0:HS.mem -> h1:HS.mem -> Lemma
+val frame_seen: #index:Type0 -> c:block index -> i:index -> l:B.loc -> s:state c i (c.state i) -> h0:HS.mem -> h1:HS.mem -> Lemma
   (requires (
     invariant c i h0 s /\
     B.loc_disjoint l (footprint c i h0 s) /\
@@ -166,7 +171,7 @@ val frame_seen: #index:Type0 -> c:block index -> i:index -> l:B.loc -> s:state c
   (ensures (seen c i h0 s == seen c i h1 s))
   [ SMTPat (seen c i h1 s); SMTPat (B.modifies l h0 h1) ]
 
-val frame_freeable: #index:Type0 -> c:block index -> i:index -> l:B.loc -> s:state c i -> h0:HS.mem -> h1:HS.mem -> Lemma
+val frame_freeable: #index:Type0 -> c:block index -> i:index -> l:B.loc -> s:state c i (c.state i) -> h0:HS.mem -> h1:HS.mem -> Lemma
   (requires (
     invariant c i h0 s /\
     freeable c i h0 s /\
@@ -185,13 +190,20 @@ val index_of_state:
   c:block index ->
   i:G.erased index -> (
   let i = G.reveal i in
-  s:state c i ->
+  t:Type0 { t == c.state i } ->
+  s:state c i t ->
   Stack index
   (fun h0 -> invariant c i h0 s)
   (fun h0 i' h1 -> h0 == h1 /\ i' == i))
 
 inline_for_extraction noextract
-val create_in (#index: Type0) (c: block index) (i: index) (r: HS.rid): ST (state c i)
+val create_in:
+  #index: Type0 ->
+  c:block index ->
+  i:index ->
+  t:Type0 { t == c.state i } ->
+  r: HS.rid ->
+  ST (state c i t)
   (requires (fun _ ->
     HyperStack.ST.is_eternal_region r))
   (ensures (fun h0 s h1 ->
@@ -203,9 +215,14 @@ val create_in (#index: Type0) (c: block index) (i: index) (r: HS.rid): ST (state
     freeable c i h1 s))
 
 inline_for_extraction noextract
-val init: #index:Type0 -> c:block index -> i:G.erased index -> (
+val init:
+  #index:Type0 ->
+  c:block index ->
+  i:G.erased index -> (
   let i = G.reveal i in
-  s:state c i -> Stack unit
+  t:Type0 { t == c.state i } ->
+  s:state c i t ->
+  Stack unit
   (requires (fun h0 ->
     invariant c i h0 s))
   (ensures (fun h0 _ h1 ->
@@ -220,7 +237,7 @@ let update_pre
   #index
   (c: block index)
   (i: index)
-  (s: state c i)
+  (s: state c i (c.state i))
   (data: B.buffer uint8)
   (len: UInt32.t)
   (h0: HS.mem)
@@ -236,7 +253,7 @@ let update_post
   #index
   (c: block index)
   (i: index)
-  (s: state c i)
+  (s: state c i (c.state i))
   (data: B.buffer uint8)
   (len: UInt32.t)
   (h0 h1: HS.mem)
@@ -253,7 +270,8 @@ val update:
   c:block index ->
   i:G.erased index -> (
   let i = G.reveal i in
-  s:state c i ->
+  t:Type0 { t == c.state i } ->
+  s:state c i t ->
   data: B.buffer uint8 ->
   len: UInt32.t ->
   Stack unit
@@ -275,7 +293,8 @@ val mk_finish:
   #index:Type0 ->
   c:block index ->
   i:index ->
-  s:state c i ->
+  t:Type0 { t == c.state i } ->
+  s:state c i t ->
   dst:B.buffer uint8 { B.len dst == c.output_len i } ->
   Stack unit
     (requires fun h0 ->
@@ -297,7 +316,8 @@ val free:
   c:block index ->
   i:G.erased index -> (
   let i = G.reveal i in
-  s:state c i ->
+  t:Type0 { t == c.state i } ->
+  s:state c i t ->
   ST unit
   (requires fun h0 ->
     freeable c i h0 s /\
