providers/evercrypt/fst/EverCrypt.Hash.Incremental.fst
@@ -56,7 +56,7 @@ let evercrypt_hash: Hacl.Streaming.Interface.block Spec.Hash.Definitions.hash_al
     (fun i -> EverCrypt.Hash.free #i)
     (fun i -> EverCrypt.Hash.copy #i)
 
-let state_s = F.state_s evercrypt_hash
+let state_s a = F.state_s evercrypt_hash a (EverCrypt.Hash.state a)
 
 let freeable #a = F.freeable evercrypt_hash a
 
@@ -70,7 +70,7 @@ let hashed #a = F.seen evercrypt_hash a
 
 let hash_fits #a = F.seen_bounded evercrypt_hash a
 
-let alg_of_state = F.index_of_state evercrypt_hash
+let alg_of_state a = F.index_of_state evercrypt_hash a (EverCrypt.Hash.state a)
 
 let frame_invariant #i = F.frame_invariant evercrypt_hash i
 
@@ -78,23 +78,24 @@ let frame_hashed #i = F.frame_seen evercrypt_hash i
 
 let frame_freeable #a = F.frame_freeable evercrypt_hash a
 
-let create_in = F.create_in evercrypt_hash
+let create_in a = F.create_in evercrypt_hash a (EverCrypt.Hash.state a)
 
-let init = F.init evercrypt_hash
+let init a = F.init evercrypt_hash a (EverCrypt.Hash.state a)
+
 let update i s data len =
   let _ = allow_inversion Spec.Agile.Hash.hash_alg in
   assert_norm (pow2 61 - 1 < pow2 64);
   assert_norm (pow2 64 < pow2 125 - 1);
-  F.update evercrypt_hash i s data len
+  F.update evercrypt_hash i (EverCrypt.Hash.state i) s data len
 
 /// The wrapper pattern, to ensure that the stack-allocated state is properly
 /// monomorphized.
-let finish_md5: finish_st MD5 = F.mk_finish evercrypt_hash MD5
-let finish_sha1: finish_st SHA1 = F.mk_finish evercrypt_hash SHA1
-let finish_sha224: finish_st SHA2_224 = F.mk_finish evercrypt_hash SHA2_224
-let finish_sha256: finish_st SHA2_256 = F.mk_finish evercrypt_hash SHA2_256
-let finish_sha384: finish_st SHA2_384 = F.mk_finish evercrypt_hash SHA2_384
-let finish_sha512: finish_st SHA2_512 = F.mk_finish evercrypt_hash SHA2_512
+let finish_md5: finish_st MD5 = F.mk_finish evercrypt_hash MD5 (EverCrypt.Hash.state MD5)
+let finish_sha1: finish_st SHA1 = F.mk_finish evercrypt_hash SHA1 (EverCrypt.Hash.state SHA1)
+let finish_sha224: finish_st SHA2_224 = F.mk_finish evercrypt_hash SHA2_224 (EverCrypt.Hash.state SHA2_224)
+let finish_sha256: finish_st SHA2_256 = F.mk_finish evercrypt_hash SHA2_256 (EverCrypt.Hash.state SHA2_256)
+let finish_sha384: finish_st SHA2_384 = F.mk_finish evercrypt_hash SHA2_384 (EverCrypt.Hash.state SHA2_384)
+let finish_sha512: finish_st SHA2_512 = F.mk_finish evercrypt_hash SHA2_512 (EverCrypt.Hash.state SHA2_512)
 
 let finish a s dst =
   let a = alg_of_state a s in
@@ -106,4 +107,4 @@ let finish a s dst =
   | SHA2_384 -> finish_sha384 s dst
   | SHA2_512 -> finish_sha512 s dst
 
-let free = F.free evercrypt_hash
+let free i = F.free evercrypt_hash i (EverCrypt.Hash.state i)
